Lets take the objective function from c)
\[
\sum_{k=1}^K z_{ik} \left(
		\log \pi_k + \log \mathcal{N}\left(x_i | \mu_k, \sigma_k \right)
	\right)
\]
and lets also remember the explicit constraint that $\sum_k \pi_k = 1$. Note that we need to sum over the entire data set so we then can write the dual of the objective function:
\begin{align*}
F &= \sum_{i=1}^N \left( \sum_{k=1}^K z_{ik} \left(
		\log \pi_k + \log \mathcal{N}\left(x_i | \mu_k, \sigma_k \right)
	\right) \right) + \lambda \left( \sum_k \pi_k - 1 \right)\\
&= \sum_{i=1}^N \sum_{k=1}^K z_{ik}\log \pi_k +
	\sum_{i=1}^N \sum_{k=1}^K z_{ik} \log \mathcal{N}\left(x_i | \mu_k, \sigma_k \right)
	 + \lambda \left( \sum_k \pi_k - 1 \right)
\end{align*}
Now lets take the derivative with respect to the variables we want to update on each step and set it to zero:

a) For $\pi_k$ (refers to $\pi_k^{(t+1)}$):
\begin{align*}
\frac{\partial F}{\partial \pi_k} &= \sum_{i=1}^N z_{ik} \frac{1}{\pi_k} + 0 + \lambda = 0 
\iff \pi_k = \frac{\sum_{i=1}^N z_{ik}}{-\lambda}
\end{align*}
By using the constraint:
\begin{align*}
1 = \sum_{k=1}^K \pi_k &= \sum_{k=1}^K \frac{\sum_{i=1}^N z_{ik}}{-\lambda}\\
&= \frac{\sum_{i=1}^N \sum_{k=1}^K z_{ik}}{-\lambda}\\
&= \frac{\sum_{i=1}^N 1}{-\lambda}\\
&= \frac{N}{-\lambda}\\
\rightarrow \lambda &= -N
\end{align*}
Then
\begin{align*}
0 = \frac{\partial F}{\partial \pi_k}  &= \sum_{i=1}^N z_{ik} \frac{1}{\pi_k} + \lambda = \sum_{i=1}^N z_{ik} \frac{1}{\pi_k} - N\\
\rightarrow \pi_k^{(t+1)} &= \frac{1}{N}\sum_{i=1}^N z_{ik}
\end{align*}

\pagebreak

\newcommand{\gaussian}{
	\left(2\pi \sigma_k^2\right)^{-\frac{1}{2}} \exp \left(
			-\frac{1}{2\sigma_k^2} \left( x_i - \mu_k \right)^2
		\right)
}

b) For $\mu_k$:\\
\begin{align*}
0 &= \frac{\partial F}{\partial \mu_k}\\
&=  \frac{\partial}{\partial \mu_k} \left( \sum_{i=1}^N \sum_{k=1}^K z_{ik}\log \pi_k +
	\sum_{i=1}^N \sum_{k=1}^K z_{ik} \log \mathcal{N}\left(x_i | \mu_k, \sigma_k \right)
	 + \lambda \left( \sum_k \pi_k - 1 \right) \right)\\
&= \frac{\partial}{\partial \mu_k} \left( 
	\sum_{i=1}^N \sum_{k=1}^K z_{ik} \log \mathcal{N}\left(x_i | \mu_k, \sigma_k \right)
	 + \lambda \left( \sum_k \pi_k - 1 \right) \right)\\
&= \frac{\partial}{\partial \mu_k}
	\sum_{i=1}^N z_{ik} \log \mathcal{N}\left(x_i | \mu_k, \sigma_k \right)\\
&=  \frac{\partial}{\partial \mu_k}
	\sum_{i=1}^N z_{ik} \log \gaussian\\
&=  \frac{\partial}{\partial \mu_k} \left(
	\sum_{i=1}^N z_{ik} \log \left(2\pi \sigma_k^2\right)^{-\frac{1}{2}} +
	\sum_{i=1}^N z_{ik}  \log \exp \left(
			-\frac{1}{2\sigma_k^2} \left( x_i - \mu_k \right)^2
		\right)
\right)\\
&=  \frac{\partial}{\partial \mu_k} \left(
	-\sum_{i=1}^N z_{ik} \log \left((2\pi)^{\frac{1}{2}} \sigma_k\right) +
	\sum_{i=1}^N z_{ik}  \left(
			-\frac{1}{2\sigma_k^2} \left( x_i - \mu_k \right)^2
		\right)
\right)\\
&=  \frac{\partial}{\partial \mu_k} \left(
	\sum_{i=1}^N z_{ik}  \left(
			-\frac{1}{2\sigma_k^2} \left( x_i - \mu_k \right)^2
		\right)
\right)\\
&= \sum_{i=1}^N z_{ik}  \left(
	\frac{1}{2\sigma_k^2} \left( x_i - \mu_k \right)
\right)\\
& \rightarrow \sum_{i=1}^N z_{ik}  \left( x_i - \mu_k \right) = 0\\
& \rightarrow \sum_{i=1}^N z_{ik} x_i = \sum_{i=1}^N z_{ik} \mu_k\\
& \rightarrow \mu_k = \frac{\sum_{i=1}^N z_{ik} x_i}{\sum_{i=1}^N z_{ik}}\\
& \rightarrow \mu_k =  \frac{\sum_{i=1}^N z_{ik} x_i}{N \pi_k^{(t+1)}} = \mu_k^{(t+1)}\\
\end{align*}

\pagebreak

c) For $\sigma_k$:\\
Reusing some derivations from b)
\begin{align*}
0 &= \frac{\partial}{\partial \sigma_k} \left(
	-\sum_{i=1}^N z_{ik} \log \left((2\pi)^{\frac{1}{2}} \sigma_k\right) +
	\sum_{i=1}^N z_{ik}  \left(
			-\frac{1}{2\sigma_k^2} \left( x_i - \mu_k \right)^2
		\right)
\right)\\
&= \frac{\partial}{\partial \sigma_k} \left(
	-\sum_{i=1}^N z_{ik} \log  \sigma_k +
	\sum_{i=1}^N z_{ik}  \left(
			-\frac{1}{2\sigma_k^2} \left( x_i - \mu_k \right)^2
		\right)
\right)\\
&= -\frac{1}{\sigma_k}\sum_{i=1}^N z_{ik} + \frac{1}{\sigma_k^3}\sum_{i=1}^N z_{ik} \left( x_i - \mu_k \right)^2
\end{align*}
Multiplying by $\sigma_k^3$ on both sides
\begin{align*}
0 &= -\sigma_k^2 \sum_{i=1}^N z_{ik} + \sum_{i=1}^N z_{ik} \left( x_i - \mu_k \right)^2\\
\sigma_k^2 \sum_{i=1}^N z_{ik} &= \sum_{i=1}^N z_{ik} \left( x_i - \mu_k \right)^2\\
\sigma_k^2 &= \frac{\sum_{i=1}^N z_{ik} \left( x_i - \mu_k \right)^2}{\sum_{i=1}^N z_{ik}}\\
\sigma_k^2 &= \frac{\sum_{i=1}^N z_{ik} \left( x_i - \mu_k \right)^2}{N\pi_k^{(t+1)}} = 
	\frac{\sum_{i=1}^N z_{ik} \left( x_i - \mu_k^{(t+1)} \right)^2}{N\pi_k^{(t+1)}}
\end{align*}